Almost prove ob_cycle

src/Axiomatic.v
@@ -84,6 +84,12 @@ Module Label.
     | _ => false
     end.
 
+  Definition is_barrier (label:t): bool :=
+    match label with
+    | barrier _ => true
+    | _ => false
+    end.
+
   Lemma read_is_reading ex ord loc val:
     is_reading loc (read ex ord loc val).
   Proof.
@@ -1199,22 +1205,22 @@ Module Valid.
 
   Lemma barrier_ob_po
         p exec
-        eid1 eid2 b
+        eid1 eid2
         (EX: pre_ex p exec)
         (CO2: co2 exec)
         (RF2: rf2 exec)
-        (EID1: Execution.label eid1 exec = Some (Label.barrier b))
+        (EID1: Execution.label_is exec Label.is_barrier eid1)
         (OB: exec.(Execution.ob) eid1 eid2):
     Execution.po eid1 eid2.
   Proof.
-    unfold co2, rf2 in *.
+    inv EID1. destruct l; ss. unfold co2, rf2 in *.
     obtac.
     - exploit RF2; eauto. i. des. congr.
     - exploit RF2; eauto. i. des. congr.
     - destruct l1; try congr; ss.
     - exploit CO2; eauto. i. des. congr.
-    - eapply addr_label in H1; eauto. des. inv EID0. destruct l; ss. congr.
-    - eapply data_label in H1; eauto. des. inv EID0. destruct l; ss. congr.
+    - eapply addr_label in H1; eauto. des. inv EID1. destruct l; ss. congr.
+    - eapply data_label in H1; eauto. des. inv EID1. destruct l; ss. congr.
     - eapply ctrl_is_po; eauto.
     - etrans; eauto. eapply addr_is_po; eauto.
     - etrans; eauto. eapply ctrl_is_po; eauto.
@@ -1230,16 +1236,16 @@ Module Valid.
 
   Lemma ob_barrier_ob
         p exec
-        eid1 eid2 eid3 b
+        eid1 eid2 eid3
         (PRE: pre_ex p exec)
         (CO2: co2 exec)
         (RF2: rf2 exec)
-        (EID2: Execution.label eid2 exec = Some (Label.barrier b))
+        (EID2: Execution.label_is exec Label.is_barrier eid2)
         (OB1: exec.(Execution.ob) eid1 eid2)
         (OB2: exec.(Execution.ob) eid2 eid3):
     <<OB: exec.(Execution.ob) eid1 eid3>>.
   Proof.
-    exploit barrier_ob_po; eauto. i.
+    inv EID2. destruct l; ss. exploit barrier_ob_po; eauto. i.
     unfold co2, rf2 in *. clear OB2.
     obtac.
     - exploit RF2; eauto. i. des. congr.
@@ -1247,10 +1253,10 @@ Module Valid.
     - destruct l2; try congr; ss.
     - exploit CO2; eauto. i. des. congr.
     - inv H0.
-      + eapply addr_label in H1; eauto. des. inv EID0. destruct l; ss; try congr. des; ss.
+      + eapply addr_label in H1; eauto. des. inv EID2. destruct l; ss; try congr. des; ss.
       + inv H. exploit RF2; eauto. i. des. congr.
     - inv H0.
-      + eapply data_label in H1; eauto. des. inv EID0. destruct l; ss. congr.
+      + eapply data_label in H1; eauto. des. inv EID2. destruct l; ss. congr.
       + inv H. exploit RF2; eauto. i. des. congr.
     - destruct l; try congr; ss.
     - destruct l; try congr; ss.
@@ -1301,6 +1307,135 @@ Module Valid.
     - exploit po_label_pre; try exact EID; eauto. i. des. congr.
   Qed.
 
+Inductive rtcn A (R: A -> A -> Prop): forall (n:nat) (a1 a2:A), Prop :=
+| rtcn_nil
+    a:
+    rtcn R 0 a a
+| rtcn_cons
+    a1 a2 a3 n
+    (A12: R a1 a2)
+    (A23: rtcn R n a2 a3):
+    rtcn R (S n) a1 a3
+.
+Hint Constructors rtcn.
+
+Lemma rtcn_rtc A (R: A -> A -> Prop) n a1 a2
+      (RTCN: rtcn R n a1 a2):
+  rtc R a1 a2.
+Proof.
+  induction RTCN; auto. econs; eauto.
+Qed.
+
+Lemma rtc_rtcn A (R: A -> A -> Prop) a1 a2
+      (RTC: rtc R a1 a2):
+  exists n, rtcn R n a1 a2.
+Proof.
+  induction RTC; eauto. i. des.
+  esplits; eauto.
+Qed.
+
+Lemma tc_rtcn A (R: A -> A -> Prop) a1 a2
+      (TC: R⁺ a1 a2):
+  exists n, rtcn R n a1 a2 /\ n > 0.
+Proof.
+  apply t_step_rt in TC. des. apply clos_rt_rt1n in TC0.
+  apply rtc_rtcn in TC0. des. esplits; eauto. lia.
+Qed.
+
+Lemma rtcn_tc A (R: A -> A -> Prop) n a1 a2
+      (RTCN: rtcn R n a1 a2)
+      (N: n > 0):
+  R⁺ a1 a2.
+Proof.
+  inv RTCN; [lia|]. apply t_step_rt. esplits; eauto.
+  apply clos_rt1n_rt. eapply rtcn_rtc. eauto.
+Qed.
+
+Lemma rtcn_snoc A (R: A -> A -> Prop) n a1 a2 a3
+      (RTCN: rtcn R n a1 a2)
+      (REL: R a2 a3):
+  rtcn R (S n) a1 a3.
+Proof.
+  revert a3 REL. induction RTCN; eauto.
+Qed.
+
+Lemma rtcn_app A (R: A -> A -> Prop) n1 n2 a1 a2 a3
+      (RTCN1: rtcn R n1 a1 a2)
+      (RTCN2: rtcn R n2 a2 a3):
+  rtcn R (n1 + n2) a1 a3.
+Proof.
+  revert n1 a1 RTCN1. induction RTCN2.
+  { i. rewrite Nat.add_0_r. ss. }
+  i. exploit rtcn_snoc; try exact A12; eauto. i.
+  exploit IHRTCN2; eauto. replace (n1 + S n) with (S n1 + n) by lia. ss.
+Qed.
+
+Lemma rtcn_inv A (R: A -> A -> Prop) n a1 a2
+      (RTCN: rtcn R n a1 a2):
+  rtcn (fun a b => R b a) n a2 a1.
+Proof.
+  induction RTCN; eauto. eapply rtcn_snoc; eauto.
+Qed.
+
+Lemma rtcn_imply
+      A (R1 R2: A -> A -> Prop) n a1 a2
+      (LE: R1 <2= R2)
+      (RTCN: rtcn R1 n a1 a2):
+  rtcn R2 n a1 a2.
+Proof.
+  induction RTCN; auto. econs; eauto.
+Qed.
+
+  Lemma minimalize_cycle
+        A a
+        (pred: A -> Prop)
+        (rel: relation A)
+        (MERGE: forall a b c, rel a b -> rel b c -> pred b -> rel a c)
+        (CYCLE: rel⁺ a a):
+    (exists a, (fun a b => rel a b /\ ~ pred a /\ ~ pred b)⁺ a a) \/
+    (exists a, pred a /\ rel a a).
+  Proof.
+    apply tc_rtcn in CYCLE. des. revert a CYCLE CYCLE0.
+    induction n using strong_nat_ind. i. rename H into IH.
+    match goal with
+    | [|- ?g] => remember g as goal eqn:GOAL; guardH GOAL
+    end.
+    assert (REDUCE: forall a, rtcn rel n a a -> pred a -> goal).
+    { i. des. inv H; [lia|]. apply rtcn_inv in A23.
+      unguardH GOAL. inv A23; eauto. apply rtcn_inv in A1.
+      exploit IH.
+      2: { econs 2; [|exact A1].  eauto. }
+      all: ss. lia.
+    }
+    destruct (classic (pred a)).
+    { eapply REDUCE; eauto. }
+    rename H into PREDA.
+    cut (goal \/ rtcn (fun a b => rel a b /\ ~ pred a /\ ~ pred b) n a a).
+    { i. des; ss. unguardH GOAL. subst. left. esplits.
+      eapply rtcn_tc; eauto.
+    }
+    cut (n <= n -> goal \/ exists b, rtcn (fun a b => rel a b /\ ~ pred a /\ ~ pred b) n a b /\ rtcn rel (n - n) b a).
+    { i. exploit H; eauto. i. des; eauto.
+      rewrite Nat.sub_diag in *. inv x0. eauto.
+    }
+    generalize n at 1 3 5 as m. induction m.
+    { right. esplits; eauto. rewrite Nat.sub_0_r. ss. }
+    i. exploit IHm; [lia|]. i. des; eauto. inv x0; [lia|].
+    replace n with (S n0 + m) in * by lia. clear H1 H CYCLE0.
+    replace (S n0 + m - S m) with n0 by lia.
+    destruct (classic (pred b)).
+    { left. eapply REDUCE; [|exact H]. eapply rtcn_app; eauto.
+      eapply rtcn_imply; [|exact x]. s. i. des. ss.
+    }
+    destruct (classic (pred a2)).
+    { left. eapply REDUCE; [|exact H0].
+      replace (S n0 + m) with (n0 + S m) by lia.
+      eapply rtcn_app; eauto. eapply rtcn_snoc; eauto.
+      eapply rtcn_imply; [|exact x]. s. i. des. ss.
+    }
+    right. esplits; eauto. eapply rtcn_snoc; eauto.
+  Qed.
+
   Lemma ob_cycle
         p exec eid
         (PRE: pre_ex p exec)
@@ -1311,10 +1446,15 @@ Module Valid.
       exists eid_nb,
         (exec.(Execution.ob) ∩ (Execution.label_is_rel exec (join Label.is_read Label.is_write)))⁺ eid_nb eid_nb>> \/
     <<BARRIER:
-      exists eid_b b,
+      exists eid_b,
         exec.(Execution.ob) eid_b eid_b /\
-        Execution.label eid_b exec = Some (Label.barrier b)>>.
+        Execution.label_is exec Label.is_barrier eid_b>>.
   Proof.
+    exploit minimalize_cycle; eauto.
+    { i. eapply ob_barrier_ob; eauto. }
+    i. des; eauto. left. esplits.
+    eapply clos_trans_mon; eauto. i. inv H. inv H1. econs; ss.
+    admit.
   Admitted.
 
   Lemma internal_rw
